wip

clightplus/compiler_proof/Clight2AsmProof.v
@@ -1,38 +1,844 @@
 From compcert Require Import Globalenvs Smallstep Simulation AST Integers Events Behaviors Errors Memory Values Maps.
 From compcert Require Import Ctypes Clight Clightdefs Globalenvs.
 Require Import ClightPlus2ClightMatchEnv.
-Require Import String.
+From Paco Require Export paco.
+Require Import String CoqlibCCR.
 
-Definition match_temps le le' := forall id, CoqlibCCR.option_rel (Val.inject inject_id) (le ! id) (le' ! id).
+Definition match_temps le le' := forall id, CoqlibCCR.option_rel Val.lessdef (le ! id) (le' ! id).
 
 Inductive match_cont : cont -> cont -> Prop :=
   | match_Kstop : match_cont Kstop Kstop
-  | match_Kseq s k k' (NEXT: match_cont k k') : match_cont (Kseq s k) (Kseq s k')
-  | match_Kloop1 s1 s2 k k' (NEXT: match_cont k k') : match_cont (Kloop1 s1 s2 k) (Kloop1 s1 s2 k')
-  | match_Kloop2 s1 s2 k k' (NEXT: match_cont k k') : match_cont (Kloop2 s1 s2 k) (Kloop2 s1 s2 k')
-  | match_Kswitch k k' (NEXT: match_cont k k') : match_cont (Kswitch k) (Kswitch k')
-  | match_Kcall id f e le le' k k' 
-      (LEINJ: match_temps le le') 
-      (NEXT: match_cont k k') 
-    : match_cont (Kcall id f e le k) (Kcall id f e le' k').
+  | match_Kseq
+        s k k'
+        (NEXT: match_cont k k') :
+      match_cont (Kseq s k) (Kseq s k')
+  | match_Kloop1
+        s1 s2 k k'
+        (NEXT: match_cont k k') :
+      match_cont (Kloop1 s1 s2 k) (Kloop1 s1 s2 k')
+  | match_Kloop2
+        s1 s2 k k'
+        (NEXT: match_cont k k') :
+      match_cont (Kloop2 s1 s2 k) (Kloop2 s1 s2 k')
+  | match_Kswitch
+        k k'
+        (NEXT: match_cont k k') :
+      match_cont (Kswitch k) (Kswitch k')
+  | match_Kcall
+        id f e le le' k k' 
+        (LEINJ: match_temps le le') 
+        (NEXT: match_cont k k') :
+      match_cont (Kcall id f e le k) (Kcall id f e le' k').
 
 Variant match_states : state -> state -> Prop :=
-  | match_state f s k k' e le le' m m' 
-      (EXT: Mem.extends m m')
-      (LEINJ: match_temps le le')
-      (NEXT: match_cont k k')
-    : match_states (State f s k e le m) (State f s k' e le' m')
-  | match_callstate fd args args' k k' m m' 
-      (EXT: Mem.extends m m')
-      (VALINJ: List.Forall2 (Val.inject inject_id) args args')
-      (NEXT: match_cont k k')
-    : match_states (Callstate fd args k m) (Callstate fd args' k' m')
-  | match_returnstate res res' k k' m m' 
-      (EXT: Mem.extends m m')
-      (VALINJ: Val.inject inject_id res res')
-      (NEXT: match_cont k k')
-    : match_states (Returnstate res k m) (Returnstate res' k' m').
+  | match_state
+        f s k k' e le le' m m' 
+        (EXT: Mem.extends m m')
+        (LEINJ: match_temps le le')
+        (NEXT: match_cont k k') :
+      match_states (State f s k e le m) (State f s k' e le' m')
+  | match_callstate
+        fd args args' k k' m m' 
+        (EXT: Mem.extends m m')
+        (VALINJ: List.Forall2 (Val.inject inject_id) args args')
+        (NEXT: match_cont k k') :
+      match_states (Callstate fd args k m) (Callstate fd args' k' m')
+  | match_returnstate
+        res res' k k' m m' 
+        (EXT: Mem.extends m m')
+        (VALINJ: Val.inject inject_id res res')
+        (NEXT: match_cont k k') :
+      match_states (Returnstate res k m) (Returnstate res' k' m').
 
+Lemma match_call_cont
+    k k'
+    (MC: match_cont k k')
+    (IS: is_call_cont k') :
+  is_call_cont k.
+Proof. unfold is_call_cont in *. des_ifs; inv MC. Qed.
+
+Lemma match_free_list
+    m m' m0 m0' l
+    (MM: Mem.extends m m')
+    (FREE: Mem.free_list m' l = Some m0')
+    (FREE0: Mem.free_list m l = Some m0) :
+  Mem.extends m0 m0'.
+Proof.
+  ginduction l; i; ss; eauto; clarify.
+  des_ifs_safe.
+  hexploit Mem.free_parallel_extends; eauto.
+  i. des. clarify. eapply IHl; eauto.
+Qed.
+
+Lemma match_free_list_match 
+    m m' m0 l
+    (MM: Mem.extends m m')
+    (FREE: Mem.free_list m l = Some m0) :
+  exists m0', Mem.free_list m' l = Some m0' /\ Mem.extends m0 m0'.
+Proof.
+  ginduction l; i; ss; clarify. { esplits; eauto. }
+  des_ifs_safe.
+  hexploit Mem.free_parallel_extends; eauto.
+  i. des. des_ifs. eapply IHl; eauto.
+Qed.
+
+(* IntPtrRel.binded_val
+(* IntptrRel.load_concrete_extends *)
+(* Mem.loadv_extends *)
+(* Mem.storev_extends *)
+Search IntPtrRel.concrete_extends.
+volatile_load *)
+
+Lemma match_sem_cast_match
+    m m' v v' ty1 ty2 v0' v0
+    (MM: Mem.extends m m')
+    (CAST: Cop.sem_cast v' ty1 ty2 m' = Some v0')
+    (CAST': Cop.sem_cast v ty1 ty2 m = Some v0)
+    (MV: Val.lessdef v v') :
+  Val.lessdef v0 v0'.
+Proof.
+  unfold Cop.sem_cast in *. des_ifs; inv MV; ss; clarify.
+Qed.
+
+Lemma match_sem_cast
+    m m' v v' ty1 ty2 v0
+    (MM: Mem.extends m m')
+    (CAST: Cop.sem_cast v ty1 ty2 m = Some v0)
+    (MV: Val.lessdef v v') :
+  exists v0', Cop.sem_cast v' ty1 ty2 m' = Some v0'.
+Proof.
+  unfold Cop.sem_cast in *. des_ifs; inv MV; ss; clarify; eauto.
+  hexploit Mem.weak_valid_pointer_extends; eauto. i. clarify.
+Qed.
+
+Lemma match_sem_un_match
+    m m' o v v' ty v0' v0
+    (MM: Mem.extends m m')
+    (OP: Cop.sem_unary_operation o v' ty m' = Some v0')
+    (OP': Cop.sem_unary_operation o v ty m = Some v0)
+    (MV: Val.lessdef v v') :
+  Val.lessdef v0 v0'.
+Proof.
+  destruct o; ss.
+  - unfold Cop.sem_notbool in *. unfold Cop.bool_val in *. des_ifs; inv MV; ss; clarify.
+  - unfold Cop.sem_notint in *. des_ifs; inv MV; ss; clarify.
+  - unfold Cop.sem_neg in *. des_ifs; inv MV; ss; clarify.
+  - unfold Cop.sem_absfloat in *. des_ifs; inv MV; ss; clarify.
+Qed.
+
+Lemma match_sem_un
+    m m' o v v' ty v0
+    (MM: Mem.extends m m')
+    (OP': Cop.sem_unary_operation o v ty m = Some v0)
+    (MV: Val.lessdef v v') :
+  exists v0', Cop.sem_unary_operation o v' ty m' = Some v0'.
+Proof.
+  destruct o; ss.
+  - unfold Cop.sem_notbool in *. unfold Cop.bool_val in *. des_ifs; inv MV; ss; clarify; eauto.
+    hexploit Mem.weak_valid_pointer_extends; eauto. i. clarify.
+  - unfold Cop.sem_notint in *. des_ifs; inv MV; ss; clarify; eauto.
+  - unfold Cop.sem_neg in *. des_ifs; inv MV; ss; clarify; eauto.
+  - unfold Cop.sem_absfloat in *. des_ifs; inv MV; ss; clarify; eauto.
+Qed.
+
+Ltac wd :=
+  match goal with
+  | H: IntPtrRel.to_ptr_val _ _ = Vlong _ |- _ => unfold IntPtrRel.to_ptr_val, Mem.to_ptr in H; des_ifs
+  | H: IntPtrRel.to_int_val _ _ = Vptr _ _ |- _ => unfold IntPtrRel.to_int_val, Mem.to_int in H; des_ifs
+  end.
+
+Ltac re :=
+  match goal with
+  | H: Int.eq _ _ = true |- _ => apply Int.same_if_eq in H
+  | H: Int64.eq _ _ = true |- _ => apply Int64.same_if_eq in H
+  | H: Ptrofs.eq _ _ = true |- _ => apply Ptrofs.same_if_eq in H
+  end.
+
+Lemma match_sem_ptr_sub_match m m' v1 v2 i
+  (MM: Mem.extends m m')
+  (OP: Cop._sem_ptr_sub_join v1 v2 m = Some i)
+:
+  Cop._sem_ptr_sub_join v1 v2 m' = Some i.
+Proof.
+  unfold Cop._sem_ptr_sub_join in OP. des_ifs.
+  - apply Ptrofs.same_if_eq in Heq1. clarify.
+    unfold Cop._sem_ptr_sub in Heq, Heq0. des_ifs; repeat wd; try solve [ss; des_ifs].
+    + repeat wd. repeat re. clarify. ss. unfold Vnullptr in *. clarify.
+      unfold IntPtrRel.to_int_val in *. ss. clarify. unfold Cop._sem_ptr_sub_join.
+      unfold IntPtrRel.to_ptr_val. ss.
+      des_ifs; unfold Cop._sem_ptr_sub in *; des_ifs.
+      { repeat re. rewrite Heq1. ss. rewrite Heq5. eauto. }
+      ss. unfold Vnullptr in *. clarify.
+    + unfold IntPtrRel.to_ptr_val, IntPtrRel.to_int_val in *.
+      unfold IntPtrRel.option_to_val in *. des_ifs.
+      hexploit (Mem.to_ptr_extends m v1 v1); eauto. i.
+      hexploit (Mem.to_ptr_extends m v2 v2); eauto. i.
+      hexploit (Mem.to_int_extends m v1 v1); eauto. i.
+      hexploit (Mem.to_int_extends m v2 v2); eauto. i. 
+      unfold Cop._sem_ptr_sub_join, Cop._sem_ptr_sub, IntPtrRel.to_int_val, IntPtrRel.to_ptr_val.
+      rewrite H, H0, H1, H2. ss. des_ifs.
+      { repeat re. f_equal. etransitivity; eauto. }
+      rewrite Heq5 in Heq7. rewrite Heq in Heq7. unfold Ptrofs.eq in Heq7. ss. des_ifs.
+  - clear Heq0. unfold Cop._sem_ptr_sub in Heq. des_ifs; repeat wd; try solve [ss; des_ifs]; ss.
+    { repeat re. unfold Vnullptr in *. clarify. }
+    unfold IntPtrRel.to_ptr_val in *.
+    unfold IntPtrRel.option_to_val in *. des_ifs.
+    hexploit (Mem.to_ptr_extends m v1 v1); eauto. i.
+    hexploit (Mem.to_ptr_extends m v2 v2); eauto. i.
+    unfold Cop._sem_ptr_sub_join, Cop._sem_ptr_sub, IntPtrRel.to_ptr_val.
+    rewrite H, H0. ss. des_ifs; try solve [repeat wd; ss; des_ifs].
+    hexploit IntPtrRel.psubl_wrapper_no_angelic.
+    { unfold IntPtrRel.to_ptr_val. rewrite H. rewrite H0. ss. }
+    { rewrite Heq4. rewrite Heq5. ss. }
+    i. ss; des; des_ifs; clarify. unfold lib.sflib.NW in *. des; clarify.
+    exfalso. hexploit Ptrofs.eq_spec. rewrite Heq3. i. apply H2. 
+    rewrite <- Ptrofs.of_int64_to_int64 at 1; ss. f_equal. apply Int64.same_if_eq.
+    unfold Int64.eq. des_ifs.
+  - clear Heq. unfold Cop._sem_ptr_sub in Heq0. des_ifs; repeat wd; try solve [ss; des_ifs]; ss.
+    unfold IntPtrRel.to_int_val, IntPtrRel.option_to_val in *. des_ifs.
+    hexploit (Mem.to_int_extends m v1 v1); eauto. i.
+    hexploit (Mem.to_int_extends m v2 v2); eauto. i.
+    unfold Cop._sem_ptr_sub_join, Cop._sem_ptr_sub, IntPtrRel.to_int_val.
+    rewrite H, H0. ss. des_ifs; try solve [re; f_equal; eauto].
+    { repeat wd. repeat re. ss. unfold Vnullptr in *. clarify. }
+    hexploit IntPtrRel.psubl_wrapper_no_angelic.
+    { rewrite Heq4. rewrite Heq5. ss. }
+    { unfold IntPtrRel.to_int_val. rewrite H. rewrite H0. ss. }
+    i. unfold lib.sflib.NW in *. ss; des; des_ifs; clarify.
+    exfalso. hexploit Ptrofs.eq_spec. rewrite Heq3. i. apply H1. 
+    rewrite <- Ptrofs.of_int64_to_int64 at 1; ss. f_equal. rewrite Heq7.
+    apply Int64.same_if_eq. unfold Int64.eq. des_ifs.
+Qed.
+
+Lemma match_sem_ptr_cmp_match m m' o v1 v2 v
+  (MM: Mem.extends m m')
+  (OP: Cop.cmp_ptr_join_common m o v1 v2 = Some v)
+:
+  exists v', Cop.cmp_ptr_join_common m' o v1 v2 = Some v' /\ Val.lessdef v v'.
+Proof.
+  unfold Cop.cmp_ptr_join_common in OP. des_ifs.
+  - unfold Cop.cmp_ptr in *. des_ifs. ss. clarify. ss.
+    unfold Cop.cmp_ptr in *. ss. clarify. ss. esplits; eauto.
+  - unfold Cop.cmp_ptr in *. des_ifs. ss. clarify. ss.
+    unfold Cop.cmp_ptr in *. ss. clarify. ss. esplits; eauto.
+    des_ifs.
+    hexploit Mem.weak_valid_pointer_extends; eauto. i. unfold Mem.weak_valid_pointer in *.
+    clarify.
+  - unfold Cop.cmp_ptr_join in *. des_ifs.
+    + re. clarify. unfold Cop.cmp_ptr in *. des_ifs. unfold Val.cmplu_bool in *.
+      des_ifs.
+      * apply andb_prop in Heq8. destruct Heq8. unfold IntPtrRel.to_ptr_val, IntPtrRel.option_to_val in *. des_ifs.
+        hexploit Mem.weak_valid_pointer_extends; eauto. i.
+        hexploit Mem.weak_valid_pointer_extends; eauto. i.
+        hexploit Mem.to_ptr_extends. 3: et. all: et. i.
+        hexploit Mem.to_ptr_extends. 3: apply Heq6. all: et. i.
+        unfold Cop.cmp_ptr_join_common in *. rewrite Heq.
+        unfold Cop.cmp_ptr_join in *. unfold IntPtrRel.to_ptr_val. rewrite H3, H4. ss.
+        clear Heq6 H4. unfold Cop.cmp_ptr, Val.cmplu_bool. 
+        unfold Mem.weak_valid_pointer in H1. des_ifs.
+        all: try solve [unfold Val.of_bool in *; ss; des_ifs].
+        all: re; clarify; try solve [esplits; et].
+        all: unfold IntPtrRel.to_int_val, IntPtrRel.option_to_val in *; des_ifs.
+        all: hexploit (Mem.to_int_extends m (Vlong i) (Vlong i)); et; i.
+        all: hexploit (Mem.to_int_extends m (Vptr b0 i5) (Vptr b0 i5)); et; i.
+        all: rewrite H in *; rewrite H4 in *; clarify; ss; clarify; red in H; clarify.
+        rewrite H7 in *. clarify. unfold Int.eq in Heq6. des_ifs.
+      * apply andb_prop in Heq8. destruct Heq8. unfold IntPtrRel.to_ptr_val, IntPtrRel.to_int_val, IntPtrRel.option_to_val in *. des_ifs.
+        hexploit Mem.weak_valid_pointer_extends; eauto. i.
+        hexploit Mem.weak_valid_pointer_extends; eauto. i.
+        hexploit Mem.to_ptr_extends. 3: et. all: et. i.
+        hexploit Mem.to_ptr_extends. 3: apply Heq6. all: et. i.
+        hexploit (Mem.to_int_extends m (Vlong i) (Vlong i)); et; i.
+        hexploit (Mem.to_int_extends m (Vptr b i0) (Vptr b i0)); et; i.
+        unfold lib.sflib.NW in *.
+        unfold Cop.cmp_ptr_join_common in *. rewrite Heq.
+        unfold Cop.cmp_ptr_join, Cop.cmp_ptr, Val.cmplu_bool, IntPtrRel.to_int_val, IntPtrRel.to_ptr_val, IntPtrRel.option_to_val in *.
+        unfold Mem.weak_valid_pointer in *. des_ifs.
+        all: try solve [esplits; et]. unfold Int.eq in Heq10. des_ifs.
+      * bsimpl. des.
+        hexploit Mem.valid_pointer_extends; eauto. i.
+        hexploit Mem.valid_pointer_extends; eauto. i.
+        unfold IntPtrRel.to_ptr_val, IntPtrRel.to_int_val, IntPtrRel.option_to_val in *. des_ifs.
+        hexploit (Mem.to_ptr_extends m (Vlong i) (Vlong i)); et; i.
+        hexploit (Mem.to_ptr_extends m (Vptr b i0) (Vptr b i0)); et; i.
+        hexploit (Mem.to_int_extends m (Vlong i) (Vlong i)); et; i.
+        hexploit (Mem.to_int_extends m (Vptr b i0) (Vptr b i0)); et; i.
+        unfold lib.sflib.NW in *.
+        unfold Cop.cmp_ptr_join_common in *. rewrite Heq.
+        unfold Cop.cmp_ptr_join, Cop.cmp_ptr, Val.cmplu_bool, IntPtrRel.to_int_val, IntPtrRel.to_ptr_val, IntPtrRel.option_to_val in *.
+        des_ifs.
+        all: try solve [esplits; et]. unfold Int.eq in Heq12. des_ifs.
+      * apply andb_prop in Heq9. des. apply andb_prop in Heq6. des.
+        hexploit Mem.weak_valid_pointer_extends; eauto. i.
+        hexploit (Mem.weak_valid_pointer_extends m m' b1); eauto. i.
+        unfold IntPtrRel.to_ptr_val, IntPtrRel.to_int_val, IntPtrRel.option_to_val in *. des_ifs.
+        hexploit (Mem.to_ptr_extends m (Vlong i) (Vlong i)); et; i.
+        hexploit (Mem.to_ptr_extends m (Vptr b i0) (Vptr b i0)); et; i.
+        hexploit (Mem.to_int_extends m (Vlong i) (Vlong i)); et; i.
+        hexploit (Mem.to_int_extends m (Vptr b i0) (Vptr b i0)); et; i.
+        unfold lib.sflib.NW in *.
+        repeat re. clarify.
+        unfold Cop.cmp_ptr_join_common in *. rewrite Heq.
+        unfold Mem.weak_valid_pointer in *.
+        unfold Cop.cmp_ptr_join, Cop.cmp_ptr, Val.cmplu_bool, IntPtrRel.to_int_val, IntPtrRel.to_ptr_val, IntPtrRel.option_to_val in *.
+        des_ifs.
+        all: try solve [esplits; et].
+        unfold Int.eq in Heq9. des_ifs.
+      * apply andb_prop in Heq9. des. apply andb_prop in Heq6. des.
+        hexploit (Mem.weak_valid_pointer_extends m m' b2); eauto. i.
+        hexploit (Mem.weak_valid_pointer_extends m m' b2 (Ptrofs.unsigned i4)); eauto. i.
+        hexploit (Mem.weak_valid_pointer_extends m m' b0); eauto. i.
+        unfold IntPtrRel.to_ptr_val, IntPtrRel.to_int_val, IntPtrRel.option_to_val in *. des_ifs.
+        hexploit (Mem.to_ptr_extends m (Vlong i) (Vlong i)); et; i.
+        hexploit (Mem.to_ptr_extends m (Vptr b i0) (Vptr b i0)); et; i.
+        hexploit (Mem.to_int_extends m (Vlong i) (Vlong i)); et; i.
+        hexploit (Mem.to_int_extends m (Vptr b i0) (Vptr b i0)); et; i.
+        unfold lib.sflib.NW in *.
+        repeat re. clarify.
+        unfold Cop.cmp_ptr_join_common in *. rewrite Heq.
+        unfold Mem.weak_valid_pointer in *.
+        unfold Cop.cmp_ptr_join, Cop.cmp_ptr, Val.cmplu_bool, IntPtrRel.to_int_val, IntPtrRel.to_ptr_val, IntPtrRel.option_to_val in *.
+        des_ifs. all: try solve [esplits; et].
+        unfold Int.eq in Heq13. des_ifs.
+      * apply andb_prop in Heq9. des. apply andb_prop in Heq6. des.
+        hexploit (Mem.weak_valid_pointer_extends m m' b0); eauto. i.
+        hexploit (Mem.valid_pointer_extends m m' b1); eauto. i.
+        hexploit (Mem.valid_pointer_extends m m' b2); eauto. i.
+        unfold IntPtrRel.to_ptr_val, IntPtrRel.to_int_val, IntPtrRel.option_to_val in *. des_ifs.
+        hexploit (Mem.to_ptr_extends m (Vlong i) (Vlong i)); et; i.
+        hexploit (Mem.to_ptr_extends m (Vptr b i0) (Vptr b i0)); et; i.
+        hexploit (Mem.to_int_extends m (Vlong i) (Vlong i)); et; i.
+        hexploit (Mem.to_int_extends m (Vptr b i0) (Vptr b i0)); et; i.
+        unfold lib.sflib.NW in *. repeat re. clarify.
+        unfold Cop.cmp_ptr_join_common in *. rewrite Heq.
+        unfold Mem.weak_valid_pointer in *.
+        unfold Cop.cmp_ptr_join, Cop.cmp_ptr, Val.cmplu_bool, IntPtrRel.to_int_val, IntPtrRel.to_ptr_val, IntPtrRel.option_to_val in *.
+        des_ifs. all: try solve [esplits; et].
+        unfold Int.eq in Heq13. des_ifs.
+    + clear Heq1. unfold Cop.cmp_ptr in *. des_ifs. unfold Val.cmplu_bool in *. des_ifs.
+      * apply andb_prop in Heq5. des.
+        hexploit (Mem.weak_valid_pointer_extends m m' b0); eauto. i.
+        unfold IntPtrRel.to_ptr_val, IntPtrRel.option_to_val in *. des_ifs.
+        hexploit (Mem.to_ptr_extends m (Vlong i) (Vlong i)); et; i.
+        hexploit (Mem.to_ptr_extends m (Vptr b i0) (Vptr b i0)); et; i.
+        unfold lib.sflib.NW in *. repeat re. clarify.
+        unfold Cop.cmp_ptr_join_common in *. rewrite Heq.
+        unfold Mem.weak_valid_pointer in *.
+        unfold Cop.cmp_ptr_join, Val.cmplu_bool, IntPtrRel.to_ptr_val, IntPtrRel.option_to_val in *.
+        unfold Cop.cmp_ptr at 1.
+        des_ifs. all: try solve [ss; clarify; des_ifs].
+      * apply andb_prop in Heq5. des.
+        hexploit (Mem.weak_valid_pointer_extends m m' b1 (Ptrofs.unsigned i2)); eauto. i.
+        hexploit (Mem.weak_valid_pointer_extends m m' b1 (Ptrofs.unsigned i3)); eauto. i.
+        unfold IntPtrRel.to_ptr_val, IntPtrRel.option_to_val in *. des_ifs.
+        hexploit (Mem.to_ptr_extends m (Vlong i) (Vlong i)); et; i.
+        hexploit (Mem.to_ptr_extends m (Vptr b i0) (Vptr b i0)); et; i.
+        unfold lib.sflib.NW in *.
+        unfold Cop.cmp_ptr_join_common in *. rewrite Heq.
+        unfold Mem.weak_valid_pointer in *.
+        unfold Cop.cmp_ptr_join, Val.cmplu_bool, IntPtrRel.to_ptr_val, IntPtrRel.option_to_val in *.
+        unfold Cop.cmp_ptr at 1.
+        des_ifs. all: try solve [ss; clarify; des_ifs].
+        all: try solve [unfold Val.of_bool in *; ss; des_ifs].
+        { unfold Cop.cmp_ptr in *. unfold Val.of_bool in *. ss. des_ifs; ss; clarify; des_ifs. }
+        { esplits; et. re. clarify. ss. des_ifs. ss. clarify. rewrite H2 in *. clarify. }
+        { unfold Coqlib.option_map in Heq2. des_ifs. unfold Cop.cmp_ptr, Coqlib.option_map in Heq8. des_ifs.
+          hexploit IntPtrRel.cmplu_no_angelic. 2:et. { unfold IntPtrRel.to_ptr_val. rewrite Heq10. rewrite Heq11. et. }
+          i. rewrite H1 in *. rewrite H2 in *. clarify. unfold Int.eq in *. des_ifs. }
+        { unfold Cop.cmp_ptr in *. unfold Val.of_bool in *. ss. des_ifs; ss; clarify; des_ifs. }
+        { unfold Cop.cmp_ptr in *. unfold Val.of_bool in *. ss. des_ifs; ss; clarify; des_ifs. }
+        { unfold Cop.cmp_ptr in *. unfold Val.of_bool in *. ss. des_ifs; ss; clarify; des_ifs. }
+        { unfold Cop.cmp_ptr in *. unfold Val.of_bool in *. ss. des_ifs; ss; clarify; des_ifs. }
+        esplits; et.
+        unfold Coqlib.option_map in Heq2. des_ifs. clear Heq8. ss. des_ifs. rewrite H3 in *.
+        clarify.
+      * bsimpl. des.
+        hexploit (Mem.valid_pointer_extends m m' b0); eauto. i.
+        hexploit (Mem.valid_pointer_extends m m' b1); eauto. i.
+        unfold IntPtrRel.to_ptr_val, IntPtrRel.option_to_val in *. des_ifs.
+        hexploit (Mem.to_ptr_extends m (Vlong i) (Vlong i)); et; i.
+        hexploit (Mem.to_ptr_extends m (Vptr b i0) (Vptr b i0)); et; i.
+        unfold lib.sflib.NW in *.
+        unfold Cop.cmp_ptr_join_common in *. rewrite Heq.
+        unfold Cop.cmp_ptr_join, Cop.cmp_ptr in *.
+        des_ifs.
+        all: try solve [unfold Val.of_bool, Coqlib.option_map in *; ss; des_ifs].
+        { re. clarify. clear Heq8. unfold IntPtrRel.to_ptr_val in Heq2 at 1.
+          rewrite H1 in Heq2. clear Heq3 H1. ss. des_ifs. esplits; et. }
+        { unfold Coqlib.option_map in *. des_ifs. hexploit IntPtrRel.cmplu_no_angelic; et.
+          i. rewrite H3 in *. rewrite H4 in *. clarify. unfold Int.eq in *. des_ifs. }
+        { clear Heq8. unfold IntPtrRel.to_ptr_val in Heq2 at 1.
+          rewrite H1 in Heq2. clear Heq3 H1. ss. des_ifs. esplits; et. }
+        { clear Heq8. unfold IntPtrRel.to_ptr_val in Heq2 at 1.
+          rewrite H1 in Heq2. clear Heq3 H1. ss. des_ifs. }
+        { clear Heq8. unfold IntPtrRel.to_ptr_val in Heq2 at 1.
+          rewrite H1 in Heq2. clear Heq3 H1. ss. des_ifs. }
+    + clear Heq0. unfold Cop.cmp_ptr in *. des_ifs. unfold Val.cmplu_bool in *. des_ifs.
+      * unfold IntPtrRel.to_int_val, IntPtrRel.option_to_val in *. des_ifs.
+        hexploit (Mem.to_int_extends m (Vlong i) (Vlong i)); et; i.
+        hexploit (Mem.to_int_extends m (Vptr b i0) (Vptr b i0)); et; i.
+        unfold lib.sflib.NW in *.
+        unfold Cop.cmp_ptr_join_common in *. rewrite Heq.
+        unfold Cop.cmp_ptr_join, Val.cmplu_bool, IntPtrRel.to_int_val, IntPtrRel.option_to_val in *.
+        unfold Cop.cmp_ptr at 2.
+        des_ifs.
+        all: try solve [unfold Cop.cmp_ptr, Val.of_bool, Coqlib.option_map in *; ss; des_ifs].
+        { re. clarify. clear Heq2. ss. rewrite Heq1 in *. clarify. esplits; et. }
+        { unfold Cop.cmp_ptr in *. des_ifs. unfold Coqlib.option_map in *. des_ifs.
+          hexploit IntPtrRel.cmplu_no_angelic; et. unfold IntPtrRel.to_int_val at 2. rewrite Heq8.
+          et. i. rewrite H in *. ss. clarify. rewrite H2 in *. clarify. unfold Int.eq in *. des_ifs. }
+        { clear Heq2. unfold Cop.cmp_ptr in *. des_ifs. ss. clarify. rewrite H0 in *. clarify. esplits; et. }
+      * apply andb_prop in Heq5. des.
+        hexploit (Mem.weak_valid_pointer_extends m m' b0); eauto. i.
+        unfold IntPtrRel.to_int_val, IntPtrRel.option_to_val in *. des_ifs.
+        hexploit (Mem.to_int_extends m (Vlong i) (Vlong i)); et; i.
+        hexploit (Mem.to_int_extends m (Vptr b i0) (Vptr b i0)); et; i.
+        unfold lib.sflib.NW in *.
+        unfold Cop.cmp_ptr_join_common in *. rewrite Heq.
+        unfold Mem.weak_valid_pointer in *.
+        unfold Cop.cmp_ptr_join, Val.cmplu_bool, IntPtrRel.to_int_val, IntPtrRel.option_to_val in *.
+        unfold Cop.cmp_ptr at 2 3.
+        des_ifs. 
+        all: try solve [unfold Cop.cmp_ptr, Val.of_bool, Coqlib.option_map in *; ss; des_ifs].
+  - unfold Cop.cmp_ptr_join in *. des_ifs. clear Heq0.
+    unfold Cop.cmp_ptr in *. des_ifs. unfold Coqlib.option_map in *. des_ifs.
+    unfold Val.cmplu_bool in *. des_ifs.
+  - re. clarify. ss. des_ifs. unfold Cop.cmp_ptr, Coqlib.option_map in OP. des_ifs.
+    unfold Val.cmplu_bool in *. des_ifs. ss.
+    hexploit (Mem.weak_valid_pointer_extends); et. i.
+    unfold Cop.cmp_ptr. unfold Val.cmplu_bool.
+    unfold Mem.weak_valid_pointer in *.
+    des_ifs; ss. rewrite Heq0. ss. esplits; et.
+  - unfold Cop.cmp_ptr_join in *. des_ifs.
+    + re. clarify. unfold Cop.cmp_ptr in *. des_ifs. unfold Coqlib.option_map in *.
+      des_ifs. unfold Val.cmplu_bool in *. des_ifs.
+      * apply andb_prop in Heq7. destruct Heq7.
+        unfold IntPtrRel.to_ptr_val, IntPtrRel.to_int_val, IntPtrRel.option_to_val in *. des_ifs.
+        hexploit Mem.weak_valid_pointer_extends; eauto. i.
+        hexploit Mem.weak_valid_pointer_extends; eauto. i.
+        hexploit Mem.to_ptr_extends. 3: et. all: et. i.
+        hexploit Mem.to_ptr_extends. 3: apply Heq5. all: et. i.
+        hexploit (Mem.to_int_extends m (Vptr b i) (Vptr b i)); et; i.
+        hexploit (Mem.to_int_extends m (Vlong i0) (Vlong i0)); et; i.
+        unfold lib.sflib.NW in *. unfold Cop.cmp_ptr_join_common in *. rewrite Heq.
+        unfold Cop.cmp_ptr_join in *.
+        unfold Cop.cmp_ptr, IntPtrRel.to_ptr_val, IntPtrRel.to_ptr_val, IntPtrRel.to_int_val, IntPtrRel.option_to_val in *. des_ifs.
+        all: try solve [unfold Coqlib.option_map, Val.of_bool in *; ss; des_ifs].
+      * apply andb_prop in Heq7. destruct Heq7.
+        unfold IntPtrRel.to_ptr_val, IntPtrRel.to_int_val, IntPtrRel.option_to_val in *. des_ifs.
+        hexploit Mem.weak_valid_pointer_extends; eauto. i.
+        hexploit Mem.weak_valid_pointer_extends; eauto. i.
+        hexploit Mem.to_ptr_extends. 3: et. all: et. i.
+        hexploit Mem.to_ptr_extends. 3: apply Heq5. all: et. i.
+        hexploit (Mem.to_int_extends m (Vptr b i) (Vptr b i)); et; i.
+        hexploit (Mem.to_int_extends m (Vlong i0) (Vlong i0)); et; i.
+        unfold lib.sflib.NW in *. unfold Cop.cmp_ptr_join_common in *. rewrite Heq.
+        unfold Cop.cmp_ptr_join, Mem.weak_valid_pointer in *.
+        unfold Cop.cmp_ptr, IntPtrRel.to_ptr_val, IntPtrRel.to_ptr_val, IntPtrRel.to_int_val, IntPtrRel.option_to_val in *. des_ifs.
+        all: try solve [unfold Coqlib.option_map, Val.of_bool in *; ss; des_ifs].
+        { unfold Coqlib.option_map in *. des_ifs. re. clarify. clear Heq7. ss. clarify. rewrite H0 in *. clarify. esplits; et. }
+        { unfold Coqlib.option_map in *. des_ifs.
+          hexploit IntPtrRel.cmplu_no_angelic; unfold IntPtrRel.to_ptr_val, IntPtrRel.to_int_val.
+          rewrite Heq11, Heq12; et. rewrite Heq9, Heq10; et. i. rewrite H5 in *. rewrite H6 in *. clarify.
+          unfold Int.eq in *. des_ifs. }
+        { clear Heq3. ss. clarify. rewrite H0 in *. clarify. esplits; et. }
+      * apply andb_prop in Heq7. destruct Heq7.
+        unfold IntPtrRel.to_ptr_val, IntPtrRel.to_int_val, IntPtrRel.option_to_val in *. des_ifs.
+        hexploit Mem.valid_pointer_extends; eauto. i.
+        hexploit Mem.valid_pointer_extends; eauto. i.
+        hexploit Mem.to_ptr_extends. 3: et. all: et. i.
+        hexploit Mem.to_ptr_extends. 3: apply Heq5. all: et. i.
+        hexploit (Mem.to_int_extends m (Vptr b i) (Vptr b i)); et; i.
+        hexploit (Mem.to_int_extends m (Vlong i0) (Vlong i0)); et; i.
+        unfold lib.sflib.NW in *. unfold Cop.cmp_ptr_join_common in *. rewrite Heq.
+        unfold Cop.cmp_ptr_join, Mem.weak_valid_pointer in *.
+        unfold Cop.cmp_ptr, IntPtrRel.to_ptr_val, IntPtrRel.to_ptr_val, IntPtrRel.to_int_val, IntPtrRel.option_to_val in *. des_ifs.
+        all: try solve [unfold Coqlib.option_map, Val.of_bool in *; ss; des_ifs].
+        { unfold Coqlib.option_map in *. des_ifs. re. clarify. clear Heq8. ss. clarify. rewrite H0 in *. clarify. esplits; et. }
+        { unfold Coqlib.option_map in *. des_ifs.
+          hexploit IntPtrRel.cmplu_no_angelic; unfold IntPtrRel.to_ptr_val, IntPtrRel.to_int_val.
+          rewrite Heq12, Heq13; et. rewrite Heq10, Heq11; et. i. rewrite H5 in *. rewrite H6 in *. clarify.
+          unfold Int.eq in *. des_ifs. }
+        { clear Heq3. ss. clarify. rewrite H0 in *. clarify. esplits; et. }
+      * apply andb_prop in Heq9. destruct Heq9.
+        apply andb_prop in Heq6. destruct Heq6.
+        unfold IntPtrRel.to_ptr_val, IntPtrRel.to_int_val, IntPtrRel.option_to_val in *. des_ifs.
+        hexploit Mem.weak_valid_pointer_extends; eauto. i.
+        hexploit (Mem.weak_valid_pointer_extends m m' b3); eauto. i.
+        hexploit Mem.to_ptr_extends. 3: et. all: et. i.
+        hexploit Mem.to_ptr_extends. 3: apply Heq6. all: et. i.
+        hexploit (Mem.to_int_extends m (Vptr b i) (Vptr b i)); et; i.
+        hexploit (Mem.to_int_extends m (Vlong i0) (Vlong i0)); et; i.
+        unfold lib.sflib.NW in *. unfold Cop.cmp_ptr_join_common in *. rewrite Heq.
+        unfold Cop.cmp_ptr_join, Mem.weak_valid_pointer in *.
+        unfold Cop.cmp_ptr, IntPtrRel.to_ptr_val, IntPtrRel.to_ptr_val, IntPtrRel.to_int_val, IntPtrRel.option_to_val in *. des_ifs.
+        all: try solve [unfold Coqlib.option_map, Val.of_bool in *; ss; des_ifs].
+      * apply andb_prop in Heq9. destruct Heq9.
+        apply andb_prop in Heq6. destruct Heq6.
+        unfold IntPtrRel.to_ptr_val, IntPtrRel.to_int_val, IntPtrRel.option_to_val in *. des_ifs.
+        hexploit (Mem.weak_valid_pointer_extends m m' b4 (Ptrofs.unsigned i4)); eauto. i.
+        hexploit (Mem.weak_valid_pointer_extends m m' b4); eauto. i.
+        hexploit (Mem.weak_valid_pointer_extends m m' b2); eauto. i.
+        hexploit Mem.to_ptr_extends. 3: et. all: et. i.
+        hexploit Mem.to_ptr_extends. 3: apply Heq6. all: et. i.
+        hexploit (Mem.to_int_extends m (Vptr b i) (Vptr b i)); et; i.
+        hexploit (Mem.to_int_extends m (Vlong i0) (Vlong i0)); et; i.
+        unfold lib.sflib.NW in *. unfold Cop.cmp_ptr_join_common in *. rewrite Heq.
+        unfold Cop.cmp_ptr_join, Mem.weak_valid_pointer in *.
+        unfold Cop.cmp_ptr, IntPtrRel.to_ptr_val, IntPtrRel.to_ptr_val, IntPtrRel.to_int_val, IntPtrRel.option_to_val in *. des_ifs.
+        all: try solve [unfold Coqlib.option_map, Val.of_bool in *; ss; des_ifs].
+      * apply andb_prop in Heq9. destruct Heq9.
+        apply andb_prop in Heq6. destruct Heq6.
+        unfold IntPtrRel.to_ptr_val, IntPtrRel.to_int_val, IntPtrRel.option_to_val in *. des_ifs.
+        hexploit (Mem.valid_pointer_extends m m' b3); eauto. i.
+        hexploit (Mem.valid_pointer_extends m m' b4); eauto. i.
+        hexploit (Mem.weak_valid_pointer_extends m m' b2); eauto. i.
+        hexploit Mem.to_ptr_extends. 3: et. all: et. i.
+        hexploit Mem.to_ptr_extends. 3: apply Heq6. all: et. i.
+        hexploit (Mem.to_int_extends m (Vptr b i) (Vptr b i)); et; i.
+        hexploit (Mem.to_int_extends m (Vlong i0) (Vlong i0)); et; i.
+        unfold lib.sflib.NW in *. unfold Cop.cmp_ptr_join_common in *. rewrite Heq.
+        unfold Cop.cmp_ptr_join, Mem.weak_valid_pointer in *.
+        unfold Cop.cmp_ptr, IntPtrRel.to_ptr_val, IntPtrRel.to_ptr_val, IntPtrRel.to_int_val, IntPtrRel.option_to_val in *. des_ifs.
+        all: try solve [unfold Coqlib.option_map, Val.of_bool in *; ss; des_ifs].
+    + clear Heq1. unfold Cop.cmp_ptr in *. des_ifs. unfold Coqlib.option_map in *.
+      des_ifs. unfold Val.cmplu_bool in *. des_ifs.
+      * apply andb_prop in Heq5. destruct Heq5. re. clarify.
+        unfold IntPtrRel.to_ptr_val, IntPtrRel.option_to_val in *. des_ifs.
+        hexploit Mem.weak_valid_pointer_extends; eauto. i.
+        hexploit Mem.to_ptr_extends. 3: et. all: et. i.
+        hexploit Mem.to_ptr_extends. 3: apply Heq3. all: et. i.
+        unfold lib.sflib.NW in *. unfold Cop.cmp_ptr_join_common in *. rewrite Heq.
+        unfold Cop.cmp_ptr_join in *.
+        unfold IntPtrRel.to_ptr_val, IntPtrRel.option_to_val in *.
+        unfold Cop.cmp_ptr at 1. des_ifs.
+        all: try solve [unfold Coqlib.option_map, Val.of_bool in *; ss; des_ifs].
+      * apply andb_prop in Heq5. destruct Heq5.
+        unfold IntPtrRel.to_ptr_val, IntPtrRel.option_to_val in *. des_ifs.
+        hexploit Mem.weak_valid_pointer_extends; eauto. i. move H at bottom.
+        hexploit Mem.weak_valid_pointer_extends; eauto. i.
+        hexploit Mem.to_ptr_extends. 3: et. all: et. i.
+        hexploit Mem.to_ptr_extends. 3: apply Heq3. all: et. i.
+        unfold lib.sflib.NW in *. unfold Cop.cmp_ptr_join_common in *. rewrite Heq.
+        unfold Cop.cmp_ptr_join in *.
+        unfold IntPtrRel.to_ptr_val, IntPtrRel.option_to_val in *.
+        unfold Cop.cmp_ptr at 1. des_ifs.
+        all: try solve [unfold Cop.cmp_ptr, Coqlib.option_map, Val.of_bool in *; ss; des_ifs].
+        { re. clarify. clear Heq5. ss. clarify. clear Heq8 Heq2. des_ifs.
+          ss. clarify. rewrite H0 in *. clarify. esplits; et. } 
+        { unfold Cop.cmp_ptr in *. des_ifs. unfold Coqlib.option_map in *. des_ifs.
+          hexploit IntPtrRel.cmplu_no_angelic; et. unfold IntPtrRel.to_ptr_val. rewrite Heq7, Heq8.
+          et. i. rewrite H4 in *. ss. clarify. rewrite H5 in *. clarify. unfold Int.eq in *. des_ifs. }
+        { clear Heq5. ss. clarify. des_ifs. ss. clarify. rewrite H0 in *. clarify. esplits; et. }
+        { clear -Heq0 H2 H3. ss. unfold Mem.weak_valid_pointer in *. des_ifs. }
+        { clear -Heq0 H2 H3. ss. unfold Mem.weak_valid_pointer in *. des_ifs. }
+      * bsimpl. des.
+        unfold IntPtrRel.to_ptr_val, IntPtrRel.option_to_val in *. des_ifs.
+        hexploit Mem.valid_pointer_extends; eauto. i. move Heq5 at bottom.
+        hexploit Mem.valid_pointer_extends; eauto. i.
+        hexploit Mem.to_ptr_extends. 3: et. all: et. i.
+        hexploit Mem.to_ptr_extends. 3: apply Heq3. all: et. i.
+        unfold lib.sflib.NW in *. unfold Cop.cmp_ptr_join_common in *. rewrite Heq.
+        unfold Cop.cmp_ptr_join in *.
+        unfold IntPtrRel.to_ptr_val, IntPtrRel.option_to_val in *.
+        unfold Cop.cmp_ptr at 1. des_ifs.
+        all: try solve [unfold Cop.cmp_ptr, Coqlib.option_map, Val.of_bool in *; ss; des_ifs].
+        { re. clarify. clear Heq8. ss. des_ifs. ss. unfold Coqlib.option_map in *. des_ifs. 
+          rewrite H3 in *. clarify. esplits; et. }
+        { unfold Cop.cmp_ptr in *. des_ifs. unfold Coqlib.option_map in *. des_ifs.
+          hexploit IntPtrRel.cmplu_no_angelic; et. unfold IntPtrRel.to_ptr_val. rewrite Heq11, Heq10.
+          et. i. rewrite H2 in *. ss. clarify. rewrite H3 in *. clarify. unfold Int.eq in *. des_ifs. }
+        { clear Heq8. ss. clarify. des_ifs. unfold Coqlib.option_map in *. des_ifs. rewrite H3 in *. clarify. esplits; et. }
+    + clear Heq0. unfold Cop.cmp_ptr in *. des_ifs. unfold Coqlib.option_map in *.
+      des_ifs. unfold Val.cmplu_bool in *. des_ifs.
+      * unfold IntPtrRel.to_int_val, IntPtrRel.option_to_val in *. des_ifs.
+        hexploit (Mem.to_int_extends m (Vlong i0) (Vlong i0)); et; i.
+        hexploit (Mem.to_int_extends m (Vptr b i) (Vptr b i)); et; i.
+        unfold lib.sflib.NW in *.
+        unfold Cop.cmp_ptr_join_common in *. rewrite Heq.
+        unfold Cop.cmp_ptr_join, Val.cmplu_bool, IntPtrRel.to_int_val, IntPtrRel.option_to_val in *.
+        unfold Cop.cmp_ptr at 2.
+        des_ifs.
+        all: try solve [unfold Cop.cmp_ptr, Val.of_bool, Coqlib.option_map in *; ss; des_ifs].
+        { re. clarify. clear Heq1. ss. rewrite H0 in *. clarify. esplits; et. }
+        { unfold Cop.cmp_ptr in *. des_ifs. unfold Coqlib.option_map in *. des_ifs.
+          hexploit IntPtrRel.cmplu_no_angelic; et. unfold IntPtrRel.to_int_val. rewrite Heq7, Heq6.
+          et. i. rewrite H in *. ss. clarify. rewrite H2 in *. clarify. unfold Int.eq in *. des_ifs. }
+        { clear Heq1. unfold Cop.cmp_ptr in *. des_ifs. ss. clarify. rewrite H0 in *. clarify. esplits; et. }
+      * apply andb_prop in Heq5. des.
+        hexploit (Mem.weak_valid_pointer_extends m m' b1); eauto. i.
+        unfold IntPtrRel.to_int_val, IntPtrRel.option_to_val in *. des_ifs.
+        hexploit (Mem.to_int_extends m (Vlong i0) (Vlong i0)); et; i.
+        hexploit (Mem.to_int_extends m (Vptr b i) (Vptr b i)); et; i.
+        unfold lib.sflib.NW in *.
+        unfold Cop.cmp_ptr_join_common in *. rewrite Heq.
+        unfold Mem.weak_valid_pointer in *.
+        unfold Cop.cmp_ptr_join, Val.cmplu_bool, IntPtrRel.to_int_val, IntPtrRel.option_to_val in *.
+        unfold Cop.cmp_ptr at 2 3.
+        des_ifs. 
+        all: try solve [unfold Cop.cmp_ptr, Val.of_bool, Coqlib.option_map in *; ss; des_ifs].
+  - ss. unfold Cop.cmp_ptr in OP. des_ifs. unfold Coqlib.option_map in *. des_ifs.
+    unfold Val.cmplu_bool in *. des_ifs.
+    + apply andb_prop in Heq2. des.
+      hexploit Mem.weak_valid_pointer_extends; eauto. i. move Heq2 at bottom.
+      hexploit Mem.weak_valid_pointer_extends; eauto. i.
+      unfold Cop.cmp_ptr, Val.cmplu_bool, Mem.weak_valid_pointer in *. des_ifs.
+      ss. esplits; et.
+    + bsimpl. des. 
+      hexploit Mem.valid_pointer_extends; eauto. i. move Heq2 at bottom.
+      hexploit Mem.valid_pointer_extends; eauto. i.
+      unfold Cop.cmp_ptr, Val.cmplu_bool in *. des_ifs.
+      ss. rewrite Heq0. esplits; et.
+Qed.
+
+(* TODO: integrate two kinds of lemma to forward sim-lemma *)
+
+Lemma match_sem_bin_match ce m m' o v v' ty1 ty2 v0' v0 v1
+  (MM: Mem.extends m m')
+  (OP': Cop.sem_binary_operation ce o v ty1 v0 ty2 m = Some v1)
+  (MV: Val.lessdef v v')
+  (MV': Val.lessdef v0 v0')
+:
+  exists v1', Cop.sem_binary_operation ce o v' ty1 v0' ty2 m' = Some v1' /\ Val.lessdef v1 v1'.
+Proof.
+  destruct o; ss.
+  - unfold Cop.sem_add in *. des_ifs; inv MV; inv MV'; ss; clarify; try rewrite OP'; eauto.
+    + unfold Cop.sem_add_ptr_int in *. des_ifs.
+    + unfold Cop.sem_add_ptr_long in *. des_ifs.
+    + unfold Cop.sem_add_ptr_int in *. des_ifs.
+    + unfold Cop.sem_add_ptr_long in *. des_ifs.
+    + unfold Cop.sem_binarith in OP'. des_ifs; ss.
+      all: hexploit (match_sem_cast m m' v' v'); eauto; i; des.
+      all: hexploit (match_sem_cast m m' v0' v0'); eauto; i; des.
+      all: unfold Cop.sem_binarith; des_ifs; ss; try rewrite H in *; try rewrite H0 in *; clarify.
+      all: try rewrite Heq2 in *; ss; clarify.
+      all: hexploit (match_sem_cast_match m m' v' v'); eauto; i.
+      all: hexploit (match_sem_cast_match m m' v0' v0'); eauto; i.
+      all: try solve [inv H1|inv H2].
+      all: inv H1; inv H2; esplits; eauto.
+    + unfold Cop.sem_binarith in OP'. des_ifs; ss.
+      all: unfold Cop.sem_cast in Heq1; des_ifs.
+    + unfold Cop.sem_binarith in OP'. des_ifs; ss.
+      all: unfold Cop.sem_cast in Heq0; des_ifs.
+    + unfold Cop.sem_binarith in OP'. des_ifs; ss.
+      all: unfold Cop.sem_cast in Heq1; des_ifs.
+  - unfold Cop.sem_sub in *. des_ifs; inv MV; inv MV'; ss; clarify; try solve [esplits; eauto].
+    + unfold Cop._sem_ptr_sub_join_common in *. des_ifs; try solve [esplits; eauto].
+      all: hexploit match_sem_ptr_sub_match; eauto; i; clarify; esplits; eauto.
+    + unfold Cop._sem_ptr_sub_join_common in *. des_ifs; try solve [esplits; eauto].
+      all: hexploit match_sem_ptr_sub_match; eauto; i; clarify; esplits; eauto.
+    + unfold Cop._sem_ptr_sub_join_common in *. des_ifs; try solve [esplits; eauto].
+      all: hexploit match_sem_ptr_sub_match; eauto; i; clarify; esplits; eauto.
+    + unfold Cop._sem_ptr_sub_join_common in *. des_ifs; try solve [esplits; eauto].
+      all: hexploit match_sem_ptr_sub_match; eauto; i; clarify; esplits; eauto.
+    + unfold Cop.sem_binarith in OP'. des_ifs.
+      all: hexploit (match_sem_cast m m' v' v'); eauto; i; des.
+      all: hexploit (match_sem_cast m m' v0' v0'); eauto; i; des.
+      all: unfold Cop.sem_binarith; des_ifs; ss; try rewrite H in *; try rewrite H0 in *; clarify.
+      all: try rewrite Heq2 in *; ss; clarify.
+      all: hexploit (match_sem_cast_match m m' v' v'); eauto; i.
+      all: hexploit (match_sem_cast_match m m' v0' v0'); eauto; i.
+      all: try solve [inv H|inv H0].
+      all: inv H; inv H0; esplits; eauto.
+    + unfold Cop.sem_binarith in OP'. des_ifs.
+      all: unfold Cop.sem_cast in Heq1; des_ifs.
+    + unfold Cop.sem_binarith in OP'. des_ifs.
+      all: unfold Cop.sem_cast in Heq0; des_ifs.
+    + unfold Cop.sem_binarith in OP'. des_ifs.
+      all: unfold Cop.sem_cast in Heq0; des_ifs.
+  - unfold Cop.sem_mul in *. des_ifs; inv MV; inv MV'; ss; clarify.
+    + unfold Cop.sem_binarith in OP'. des_ifs; ss.
+      all: hexploit (match_sem_cast m m' v' v'); eauto; i; des.
+      all: hexploit (match_sem_cast m m' v0' v0'); eauto; i; des.
+      all: unfold Cop.sem_binarith; des_ifs; ss; try rewrite H in *; try rewrite H0 in *; clarify.
+      all: try rewrite Heq1 in *; ss; clarify.
+      all: hexploit (match_sem_cast_match m m' v' v'); eauto; i.
+      all: hexploit (match_sem_cast_match m m' v0' v0'); eauto; i.
+      all: try solve [inv H1|inv H2].
+      all: inv H1; inv H2; esplits; eauto.
+    + unfold Cop.sem_binarith in OP'. des_ifs.
+      all: unfold Cop.sem_cast in Heq0; des_ifs.
+    + unfold Cop.sem_binarith in OP'. des_ifs.
+      all: unfold Cop.sem_cast in Heq; des_ifs.
+    + unfold Cop.sem_binarith in OP'. des_ifs.
+      all: unfold Cop.sem_cast in Heq0; des_ifs.
+  - unfold Cop.sem_div in *. des_ifs; inv MV; inv MV'; ss; clarify.
+    + unfold Cop.sem_binarith in OP'. des_ifs; ss.
+      all: hexploit (match_sem_cast m m' v' v'); eauto; i; des.
+      all: hexploit (match_sem_cast m m' v0' v0'); eauto; i; des.
+      all: unfold Cop.sem_binarith; des_ifs; ss; try rewrite H in *; try rewrite H0 in *; clarify.
+      all: try rewrite Heq1 in *; ss; clarify.
+      all: hexploit (match_sem_cast_match m m' v' v'); eauto; i.
+      all: hexploit (match_sem_cast_match m m' v0' v0'); eauto; i.
+      all: try solve [inv H1|inv H2].
+      all: inv H1; inv H2; esplits; eauto; clarify.
+    + unfold Cop.sem_binarith in OP'. des_ifs.
+      all: unfold Cop.sem_cast in Heq0; des_ifs.
+    + unfold Cop.sem_binarith in OP'. des_ifs.
+      all: unfold Cop.sem_cast in Heq; des_ifs.
+    + unfold Cop.sem_binarith in OP'. des_ifs.
+      all: unfold Cop.sem_cast in Heq0; des_ifs.
+  - unfold Cop.sem_mod in *. des_ifs; inv MV; inv MV'; ss; clarify.
+    + unfold Cop.sem_binarith in OP'. des_ifs; ss.
+      all: hexploit (match_sem_cast m m' v' v'); eauto; i; des.
+      all: hexploit (match_sem_cast m m' v0' v0'); eauto; i; des.
+      all: unfold Cop.sem_binarith; des_ifs; ss; try rewrite H in *; try rewrite H0 in *; clarify.
+      all: try rewrite Heq1 in *; ss; clarify.
+      all: hexploit (match_sem_cast_match m m' v' v'); eauto; i.
+      all: hexploit (match_sem_cast_match m m' v0' v0'); eauto; i.
+      all: try solve [inv H1|inv H2].
+      all: inv H1; inv H2; esplits; eauto; clarify.
+    + unfold Cop.sem_binarith in OP'. des_ifs.
+      all: unfold Cop.sem_cast in Heq0; des_ifs.
+    + unfold Cop.sem_binarith in OP'. des_ifs.
+      all: unfold Cop.sem_cast in Heq; des_ifs.
+    + unfold Cop.sem_binarith in OP'. des_ifs.
+      all: unfold Cop.sem_cast in Heq0; des_ifs.
+  - unfold Cop.sem_and in *. des_ifs; inv MV; inv MV'; ss; clarify.
+    + unfold Cop.sem_binarith in OP'. des_ifs; ss.
+      all: hexploit (match_sem_cast m m' v' v'); eauto; i; des.
+      all: hexploit (match_sem_cast m m' v0' v0'); eauto; i; des.
+      all: unfold Cop.sem_binarith; des_ifs; ss; try rewrite H in *; try rewrite H0 in *; clarify.
+      all: try rewrite Heq1 in *; ss; clarify.
+      all: hexploit (match_sem_cast_match m m' v' v'); eauto; i.
+      all: hexploit (match_sem_cast_match m m' v0' v0'); eauto; i.
+      all: try solve [inv H1|inv H2].
+      all: inv H1; inv H2; esplits; eauto; clarify.
+    + unfold Cop.sem_binarith in OP'. des_ifs.
+      all: unfold Cop.sem_cast in Heq0; des_ifs.
+    + unfold Cop.sem_binarith in OP'. des_ifs.
+      all: unfold Cop.sem_cast in Heq; des_ifs.
+    + unfold Cop.sem_binarith in OP'. des_ifs.
+      all: unfold Cop.sem_cast in Heq0; des_ifs.
+  - unfold Cop.sem_or in *. des_ifs; inv MV; inv MV'; ss; clarify.
+    + unfold Cop.sem_binarith in OP'. des_ifs; ss.
+      all: hexploit (match_sem_cast m m' v' v'); eauto; i; des.
+      all: hexploit (match_sem_cast m m' v0' v0'); eauto; i; des.
+      all: unfold Cop.sem_binarith; des_ifs; ss; try rewrite H in *; try rewrite H0 in *; clarify.
+      all: try rewrite Heq1 in *; ss; clarify.
+      all: hexploit (match_sem_cast_match m m' v' v'); eauto; i.
+      all: hexploit (match_sem_cast_match m m' v0' v0'); eauto; i.
+      all: try solve [inv H1|inv H2].
+      all: inv H1; inv H2; esplits; eauto; clarify.
+    + unfold Cop.sem_binarith in OP'. des_ifs.
+      all: unfold Cop.sem_cast in Heq0; des_ifs.
+    + unfold Cop.sem_binarith in OP'. des_ifs.
+      all: unfold Cop.sem_cast in Heq; des_ifs.
+    + unfold Cop.sem_binarith in OP'. des_ifs.
+      all: unfold Cop.sem_cast in Heq0; des_ifs.
+  - unfold Cop.sem_xor in *. des_ifs; inv MV; inv MV'; ss; clarify.
+    + unfold Cop.sem_binarith in OP'. des_ifs; ss.
+      all: hexploit (match_sem_cast m m' v' v'); eauto; i; des.
+      all: hexploit (match_sem_cast m m' v0' v0'); eauto; i; des.
+      all: unfold Cop.sem_binarith; des_ifs; ss; try rewrite H in *; try rewrite H0 in *; clarify.
+      all: try rewrite Heq1 in *; ss; clarify.
+      all: hexploit (match_sem_cast_match m m' v' v'); eauto; i.
+      all: hexploit (match_sem_cast_match m m' v0' v0'); eauto; i.
+      all: try solve [inv H1|inv H2].
+      all: inv H1; inv H2; esplits; eauto; clarify.
+    + unfold Cop.sem_binarith in OP'. des_ifs.
+      all: unfold Cop.sem_cast in Heq0; des_ifs.
+    + unfold Cop.sem_binarith in OP'. des_ifs.
+      all: unfold Cop.sem_cast in Heq; des_ifs.
+    + unfold Cop.sem_binarith in OP'. des_ifs.
+      all: unfold Cop.sem_cast in Heq0; des_ifs.
+  - unfold Cop.sem_shl in *. des_ifs; inv MV; inv MV'; ss; clarify.
+    + unfold Cop.sem_shift in OP'. des_ifs; ss.
+      all: unfold Cop.sem_shift; des_ifs; esplits; eauto.
+    + unfold Cop.sem_shift in OP'. des_ifs; ss.
+      all: unfold Cop.sem_shift; des_ifs; esplits; eauto.
+    + unfold Cop.sem_shift in OP'. des_ifs; ss.
+      all: unfold Cop.sem_shift; des_ifs; esplits; eauto.
+    + unfold Cop.sem_shift in OP'. des_ifs; ss.
+      all: unfold Cop.sem_shift; des_ifs; esplits; eauto.
+  - unfold Cop.sem_shr in *. des_ifs; inv MV; inv MV'; ss; clarify.
+    + unfold Cop.sem_shift in OP'. des_ifs; ss.
+      all: unfold Cop.sem_shift; des_ifs; esplits; eauto.
+    + unfold Cop.sem_shift in OP'. des_ifs; ss.
+      all: unfold Cop.sem_shift; des_ifs; esplits; eauto.
+    + unfold Cop.sem_shift in OP'. des_ifs; ss.
+      all: unfold Cop.sem_shift; des_ifs; esplits; eauto.
+    + unfold Cop.sem_shift in OP'. des_ifs; ss.
+      all: unfold Cop.sem_shift; des_ifs; esplits; eauto.
+  - unfold Cop.sem_cmp in *. des_ifs; inv MV; inv MV'; ss; clarify.
+    all: try solve [eapply match_sem_ptr_cmp_match; et].
+    + unfold Cop.cmp_ptr_join_common in OP'. des_ifs.
+    + des_ifs. 
+
+    admit "".
+Qed.
+
+
+Lemma match_deref_loc_match t m m' vp vp' v v'
+  (MM: Mem.extends m m')
+  (DEREF: deref_loc t m vp v)
+  (DEREF': deref_loc t m' vp' v')
+  (MV: Val.lessdef vp vp')
+:
+  Val.lessdef v v'.
+Proof.
+  inv DEREF; inv DEREF'; ss; clarify; rewrite H in *; clarify.
+  hexploit Mem.loadv_extends; eauto. i. des. clarify. 
+Qed.
+
+Lemma match_eval_match ge e le le' m m' a
+  (MM: Mem.extends m m')
+  (MLE: match_temps le le')
+:
+  (forall v v', Clight.eval_expr ge e le m a v -> Clight.eval_expr ge e le' m' a v' -> Val.lessdef v v')
+  /\ (forall v v', Clight.eval_lvalue ge e le m a v -> Clight.eval_lvalue ge e le' m' a v' -> Val.lessdef v v').
+Proof.
+  ginduction a; i; ss; clarify.
+  all: try solve [split; i; inv H; inv H0; ss; inv H1; inv H].
+  - split; i; inv H; inv H0; ss; clarify.
+    inv H; inv H1; clarify; eapply match_deref_loc_match; eauto.
+  - split; i; inv H; inv H0; ss; clarify; try solve [inv H| inv H1].
+    specialize (MLE i). rewrite H4 in *. rewrite H3 in *. inv MLE. eauto.
+  - hexploit IHa; eauto. i. des. split; i; inv H1; inv H2; cycle 1. { hexploit H; eauto. }
+    inv H3; inv H1. hexploit H; eauto. i. hexploit match_deref_loc_match; eauto. 
+  - hexploit IHa; eauto. i. des. split; i; inv H1; inv H2; try solve [inv H1|inv H3].
+    hexploit H0; eauto.
+  - hexploit IHa; eauto. i. des. split; i; inv H1; inv H2; try solve [inv H1|inv H3].
+    hexploit H; eauto. i. hexploit match_sem_un_match; eauto.
+  - hexploit IHa1; eauto. i. des. hexploit IHa2; eauto. i. des.
+    split; i; inv H3; inv H4; try solve [inv H5|inv H3].
+    hexploit H; eauto. hexploit H1; eauto. i. hexploit match_sem_bin_match; eauto.
+  -
+    inv H3; inv H1. hexploit H; eauto. i. hexploit match_deref_loc_match; eauto. 
+  -
+      
+    
+
+Admitted.
+
+Lemma match_eval_expr_match ge e le le' m m' a
+  (MM: Mem.extends m m')
+  (MLE: match_temps le le')
+:
+  forall v', Clight.eval_expr ge e le' m' a v' -> exists v, Val.lessdef v v' /\ Clight.eval_expr ge e le m a v.
+Proof.
+  hexploit match_eval_match; eauto. i. des. eauto.
+Qed.
+
+Lemma match_eval_lvalue_match ge e le le' m m' a
+  (MM: Mem.extends m m')
+  (MLE: match_temps le le')
+:
+  forall v', Clight.eval_lvalue ge e le' m' a v' -> exists v, Val.lessdef v v' /\ Clight.eval_lvalue ge e le m a v.
+Proof.
+  hexploit match_eval_match; eauto. i. des. eauto.
+Qed.
+
+Lemma match_assign_loc_match ce m m' m0' vp vp' v v' ty
+  (MM: Mem.extends m m')
+  (CAST: assign_loc ce ty m' vp' v' m0')
+  (MV: Val.lessdef vp vp')
+  (MV': Val.lessdef v v')
+:
+  exists m0, Mem.extends m0 m0' /\ assign_loc ce ty m vp v m0.
+Proof.
+Admitted.
+  
 Lemma match_states_bsim p gmtgt st_src st_tgt
   (M: match_states st_src st_tgt)
 :
@@ -40,6 +846,62 @@ Lemma match_states_bsim p gmtgt st_src st_tgt
   (* (concrete_snapshot (Genv.globalenv p) (Callstate f [] Kstop m'))  *)
   lt 0%nat st_src st_tgt.
 Proof.
+  revert_until st_src. revert st_src. pcofix CIH.
+  i. inv M.
+  - destruct s.
+    + pfold. econs. i. rr.
+      unfold safe in *. hexploit SAFESRC. { apply star_refl. }
+      i. des. { inv H. } econs.
+      * i. left. inv STEPTGT.
+        ** inv NEXT. esplits.
+            { instantiate (1:=E0). econs. }
+            { left. apply plus_one. econs. }
+            { right. apply CIH. econs; eauto. }
+        ** inv NEXT. esplits.
+            { instantiate (1:=E0). econs. }
+            { left. apply plus_one. econs. eauto. }
+            { right. apply CIH. econs; eauto. econs; eauto. }
+        ** inv NEXT. esplits.
+            { instantiate (1:=E0). econs. }
+            { left. apply plus_one. econs. }
+            { right. apply CIH. econs; eauto. }
+        ** hexploit match_call_cont; eauto. i.
+           inv H; ss. hexploit match_free_list; eauto. i.
+           esplits.
+           { instantiate (1:=E0). econs. }
+           { left. apply plus_one. econs; eauto. }
+           { right. apply CIH. econs; eauto. }
+        ** inv NEXT. esplits.
+            { instantiate (1:=E0). econs. }
+            { left. apply plus_one. apply step_skip_break_switch. eauto. }
+            { right. apply CIH. econs; eauto. }
+      * i. inv FINALTGT.
+      * right. destruct k'.
+        ** inv NEXT. inv H. hexploit match_free_list_match; eauto.
+           i. des. esplits. apply step_skip_call; eauto.
+        ** esplits. econs.
+        ** esplits. econs. eauto.
+        ** esplits. econs.
+        ** esplits. apply step_skip_break_switch. eauto.
+        ** inv NEXT. inv H. hexploit match_free_list_match; eauto.
+           i. des. esplits. apply step_skip_call; eauto.
+    + pfold. econs. i. rr.
+      unfold safe in *. hexploit SAFESRC. { apply star_refl. }
+      i. des. { inv H. } inv H; des; clarify. econs.
+      * i. left. inv STEPTGT; des; clarify.
+        (* change to consistency lemma *)
+        hexploit match_eval_expr_match; eauto. i. des.
+        hexploit match_eval_lvalue_match; eauto. i. des.
+        hexploit match_sem_cast_match; eauto. i. des.
+        hexploit match_assign_loc_match; eauto. i. des.
+        esplits.
+        { instantiate (1:=E0). econs. }
+        { left. apply plus_one. econs; eauto. }
+        { right. apply CIH. econs; eauto. }
+      * i. inv FINALTGT.
+        (* change to progress lemma *)
+      * right. esplits.  2:{  }
+    +
 Admitted.
 
 Lemma semantics2to3 p:
